src/lowparse/LowParse.Spec.BoundedInt.fsti
@@ -199,6 +199,21 @@ val parse_bounded_int32
   (max: nat { 0 < max /\ min <= max /\ max < 4294967296 })
 : Tot (parser (parse_bounded_int32_kind max) (bounded_int32 min max))
 
+val parse_bounded_int32_eq
+  (min: nat)
+  (max: nat { 0 < max /\ min <= max /\ max < 4294967296 })
+  (input: bytes)
+: Lemma
+  (let sz = log256' max in
+   parse (parse_bounded_int32 min max) input == (
+     match parse (parse_bounded_integer sz) input with
+     | None -> None
+     | Some (x, consumed) ->
+       if in_bounds min max x
+       then Some (x, consumed)
+       else None
+   ))
+
 val serialize_bounded_int32
   (min: nat)
   (max: nat { 0 < max /\ min <= max /\ max < 4294967296 })
@@ -208,6 +223,21 @@ val parse_bounded_int32_le
   (min: nat)
   (max: nat { 0 < max /\ min <= max /\ max < 4294967296 })
 : Tot (parser (parse_bounded_int32_kind max) (bounded_int32 min max))
+
+val parse_bounded_int32_le_eq
+  (min: nat)
+  (max: nat { 0 < max /\ min <= max /\ max < 4294967296 })
+  (input: bytes)
+: Lemma
+  (let sz = log256' max in
+   parse (parse_bounded_int32_le min max) input == (
+     match parse (parse_bounded_integer_le sz) input with
+     | None -> None
+     | Some (x, consumed) ->
+       if in_bounds min max x
+       then Some (x, consumed)
+       else None
+   ))
 
 val serialize_bounded_int32_le
   (min: nat)
@@ -230,6 +260,20 @@ val parse_bounded_int32_le_fixed_size
   (min: nat)
   (max: nat { min <= max })
 : Tot (parser parse_bounded_int32_fixed_size_kind (bounded_int32 min max))
+
+val parse_bounded_int32_le_fixed_size_eq
+  (min: nat)
+  (max: nat { min <= max })
+  (input: bytes)
+: Lemma
+  (parse (parse_bounded_int32_le_fixed_size min max) input == (
+     match parse parse_u32_le input with
+     | None -> None
+     | Some (x, consumed) ->
+       if in_bounds min max x
+       then Some (x, consumed)
+       else None
+   ))
 
 val serialize_bounded_int32_le_fixed_size
   (min: nat)
